%% Geometry of circles %%
% Question 7
\hlquestion Show that the equation of the tangent at the pont ($x_{1},y_{1}$) 
on the circle 
\[ 
	x^{2} + y^{2} + 2gx + 2fy + c = 0
\]
is given by
\[ 
	x x_{1} + y y_{1} + g(x + x_{1}) + f(y + y_{1}) + c = 0
\]
% \begin{equation}
%  	x x_{1} + y y_{1} + g(x + x_{1}) + f(y + y_{1}) + c = 0
% 	\label{eq:M8_circ_q07_tangent}
% \end{equation}

\begin{solution}
	\[ 
		x^{2} + y^{2} + 2gx + 2fy + c = 0
	\]
	\[ 
		\rightarrow
		(x+g)^{2} + (y+f)^{2} = r^{2} 
		,\quad
		\text{where} \;
		r^{2} = g^{2} + f^{2} - c
	\]
	\[
		\text{centre} \; 
		( -g, -f )
		% ,\; 
		% \text{radius} = 
		% \sqrt{g^{2} + f^{2} - c}
	\]
	\underline{Step 1:} find gradient of tangent to circle at point 
	($x_{1},y_{1}$)
	\par
	\textit{Classic:}
	\newline
	For: $(-g, -f) \leftrightarrow (x_{1}, y_{1})$, using: 
	\[
		m_{1} = 
		\frac{y_{1} - y_{2}}{x_{1} - x_{2}}
		\quad
		\&
		\quad
		m_{1} m_{2} = -1
	\]
	\begin{align*}
		m_{1} 
			&= 
			\frac{-f - y_{1}}{-g - x_{1}}
			\qquad\qquad\qquad
			\text{or}
			&
			m_{1} 
				&= 
				\frac{y_{1} + f}{x_{1} + g}
			\\
		m_{2} 
			&= 
			-\left( \frac{-g - x_{1}}{-f - y_{1}} \right)
			\qquad
			&
			m_{2} 
				&= 
				- \left( \frac{x_{1} + g}{y_{1} + f} \right)
			\\
		m_{2} 
			&= 
			\frac{g + x_{1}}{-f - y_{1}}
			\qquad
			&
			m_{2} 
				&= 
				\frac{- x_{1} - g}{y_{1} + f}
	\end{align*}
	\textit{Using calculus:} 
	(BE note: more intuitive, but can't expect students to know\dots)
	\[ 
		x^{2} + y^{2} + 2gx + 2fy + c = 0
	\]
	Differentiate w.r.t. $x$
	% \[
	% 	\rightarrow
	% 	\frac{d}{dx}\left( x^{2} \right)
	% 	+
	% 	\frac{d}{dx}\left( y^{2} \right)
	% 	+
	% 	\frac{d}{dx}\left( 2gx \right)
	% 	+
	% 	\frac{d}{dx}\left( 2fy \right)
	% 	+
	% 	\frac{d}{dx}\left( c \right)
	% 	= 0
	% \]
	% \[
	% 	\rightarrow
	% 	2x
	% 	+
	% 	2y \frac{dy}{dx}
	% 	+
	% 	2g
	% 	+
	% 	2f \frac{dy}{dx}
	% 	= 0		
	% \]
	% \[
	% 	\frac{dy}{dx} (y+f)
	% 	=
	% 	-x - g		
	% \]
	% \[
	% 	m_{2}
	% 	=
	% 	\frac{dy}{dx} 
	% 	=
	% 	\frac{-x - g}{y + f}
	% \]
	\begin{align*}
		\rightarrow
		\frac{d}{dx}\left( x^{2} \right)
		+
		\frac{d}{dx}\left( y^{2} \right)
		+
		\frac{d}{dx}\left( 2gx \right)
			&+
			\frac{d}{dx}\left( 2fy \right)
			+
			\frac{d}{dx}\left( c \right)
			= 0
			\\
		\rightarrow
		2x
		+
		2y \frac{dy}{dx}
		+
		2g
		+
		2f \frac{dy}{dx}
			&= 0	
			\\
		\frac{dy}{dx} (y+f)
			&=
			-x - g
			\\
		\frac{dy}{dx} 
			&=
			\frac{-x - g}{y + f}
			\\
		\therefore
		m_{2}
			&=
			\frac{-(x_{1} + g)}{y_{1} + f}
	\end{align*}
	\underline{Step 2:} find equation of tangent to circle at point
	($x_{1},y_{1}$)
	\newline
	\textit{Check*:} 
	\\
	Using
	\[
		y = m_{2}x + c
	\]
	\[
		\rightarrow
		y_{1}
		= 
		\left( \frac{-(x_{1} + g)}{y_{1} + f} \right)x_{1}
		+ c
	\]
	\begin{align*}
		\rightarrow
		c
			&= 
			y_{1} 
			+ 
			\left( \frac{x_{1}(x_{1} + g)}{y_{1} + f} \right)
			\\
		c
			&= 
			\frac{
				\big(
					y_{1}(y_{1} + f) + x_{1}(x_{1} + g)
				\big)
			}{ 
				(y_{1} + f) 
			}
		% 	\\
		% c
		% 	&= 
		% 	\frac{1}{ (y_{1} + f) }
		% 	\bigg( 
		% 		y_{1}(y_{1} + f)
		% 		+
		% 		x_{1}(x_{1} + g)	
		% 	\bigg)
	\end{align*}
	% \( \therefore \)
	\[
		\rightarrow
		y
		=
		\left( \frac{-x (x_{1} + g)}{y_{1} + f} \right)
		+
		\left(
		\frac{
				y_{1}(y_{1} + f) + x_{1}(x_{1} + g)
			}{
				y_{1} + f
			}
		\right)
	\]
	\[
		% \rightarrow
		y (y_{1} + f)
		=
		-x (x_{1} + g)
		+
		y_{1}(y_{1} + f) 
		+ 
		x_{1}(x_{1} + g)
	\]
	\[
		y y_{1} + fy
		=
		-x x_{1} - gx
		+
		y_{1}^{2} + f y_{1}
		+ 
		x_{1}^{2} + g x_{1}
	\]
	\begin{equation}
		y y_{1} + x x_{1}
		+ fy - f y_{1}
		+ gx - g x_{1}
		- x_{1}^{2} 
		- y_{1}^{2}  
		= 0
		\label{eq:M8_circ_q07_expanded_tangent_1}
	\end{equation}
	\textit{Alt: }
	\\
	Using
	\[
		y - y_{1} = m (x - x_{1})
		% y = m_{2}x + c
	\]
	\[
		\rightarrow
		y - y_{1}
		= 
		\left( \frac{-(x_{1} + g)}{y_{1} + f} \right)
		(x - x_{1})
	\]
	\[
		(y - y_{1})(y_{1} + f)
		= 
		-(x_{1} + g)(x - x_{1})
	\]
	\[
		(y - y_{1})(y_{1} + f)
		+
		(x_{1} + g)(x - x_{1})
		= 0
	\]
	% \[
	% 	y y_{1} - y_{1}^{2} + fy - fy_{1}
	% 	= 
	% 	-x x_{1} - gx + x_{1}^{2} + gx_{1}
	% \]
	\[
		y y_{1} - y_{1}^{2} + fy - fy_{1}
		+ 
		x x_{1} - x_{1}^{2} + gx - gx_{1}
		= 0 
	\]
	\begin{equation}
		y y_{1} 
		+ 
		x x_{1}  
		+ fy - fy_{1}
		+ gx - gx_{1} 
		- x_{1}^{2}
		- y_{1}^{2} 
		= 0 
		\tag{\ref{eq:M8_circ_q07_expanded_tangent_1}}
	\end{equation}
	Don't simplify yet - need the c term!
	\newline
	We know that all points on the circle [including ($x_{1},y_{1}$)] satisfy:
	\begin{align*}
		x^{2} + y^{2} + 2gx + 2fy + c 
			&= 0
			\\
		\rightarrow
			x_{1}^{2} + y_{1}^{2} + 2gx_{1} + 2fy_{1} + c 
			&= 0
	\end{align*}
	\begin{equation}
		x_{1}^{2} + y_{1}^{2} + gx_{1} + fy_{1} 
		=
		-gx_{1} -fy_{1} - c
		\label{eq:M8_circ_q07_rearranged_circle_eq}
	\end{equation}
	Rearranging (\ref{eq:M8_circ_q07_expanded_tangent_1})
	\begin{equation}
		\rightarrow
		y y_{1} + x x_{1} + fy + gx 
		=
		fy_{1} + gx_{1} + x_{1}^{2} + y_{1}^{2}
		\label{eq:M8_circ_q07_expanded_tangent_2}
	\end{equation}
	We know that all points on circle meet criteria in 
	(\ref{eq:M8_circ_q07_rearranged_circle_eq})\dots
	\newline
	$\rightarrow$ sub (\ref{eq:M8_circ_q07_rearranged_circle_eq})
	into (\ref{eq:M8_circ_q07_expanded_tangent_2})
	\[
		\rightarrow
		y y_{1} + x x_{1} + fy + gx 
		=
		-gx_{1} -fy_{1} - c
	\]
	\[
		\rightarrow
		y y_{1} 
		+ 
		x x_{1} 
		+ 
		fy 
		+ 
		gx
		+
		gx_{1}
		+ 
		fy_{1} 
		+
		c 
		= 0
	\]
	\[
		x x_{1} + y y_{1} 
		+ gx + gx_{1}
		+ fy + fy_{1} 
		+ c 
		= 0
	\]
	\[
		\underline{
			x x_{1} + y y_{1} 
			+ g(x + x_{1})
			+ f(y + y_{1})
			+ c 
			= 0
		}
	\]
	Desmos calculator:
	\url{https://www.desmos.com/calculator/xu8w1xn8ho} 
	% \qSol{$\therefore$ x = 1}{}
\end{solution}

\appenddata{questionSolutions}{
{
	No solution (proof).
}
}